Add proofs for MLDSA portable sample functions

libcrux-ml-dsa/src/simd/portable/sample.rs
@@ -1,95 +1,207 @@
-use crate::{constants::FIELD_MODULUS, helper::cloop};
+use crate::constants::FIELD_MODULUS;
 
+#[hax_lib::fstar::before(
+r#"#push-options "--z3rlimit 1500 --max_fuel 3 --max_ifuel 3 --ext context_pruning --z3refresh"
+
+let rejection_sample_coefficient_lemma (randomness:Seq.seq u8) (i:nat{i < (Seq.length randomness) / 3}) :
+  Lemma (let b0 = cast (Seq.index randomness (i * 3)) <: i32 in
+        let b1 = cast (Seq.index randomness (i * 3 + 1)) <: i32 in
+        let b2 = cast (Seq.index randomness (i * 3 + 2)) <: i32 in
+        let coefficient = (((b2 <<! mk_i32 16) |. (b1 <<! mk_i32 8)) |. b0) &.
+            mk_i32 8388607 in
+        Spec.MLDSA.Math.rejection_sample_coefficient randomness i == coefficient) =
+  let b0 = cast (Seq.index randomness (i * 3)) <: i32 in
+  let b1 = cast (Seq.index randomness (i * 3 + 1)) <: i32 in
+  let b2 = cast (Seq.index randomness (i * 3 + 2)) <: i32 in
+  let b2' = if b2 >. mk_i32 127 then b2 -. mk_i32 128  else b2 in
+  assert_norm (pow2 23 == 8388608);
+  assert (b2' == (b2 %! mk_i32 128));
+  assert (((mk_i32 (pow2 16) *. b2) %! mk_i32 (pow2 23)) == (mk_i32 (pow2 16) *. (b2 %! mk_i32 128)));
+  logor_disjoint (b2 <<! mk_i32 16) (b1 <<! mk_i32 8) 16;
+  assert (((b2 <<! mk_i32 16) |. (b1 <<! mk_i32 8)) == ((b2 <<! mk_i32 16) +. (b1 <<! mk_i32 8)));
+  logor_disjoint ((b2 <<! mk_i32 16) |. (b1 <<! mk_i32 8)) b0 8;
+  assert ((((b2 <<! mk_i32 16) |. (b1 <<! mk_i32 8)) |. b0) ==
+    (((b2 <<! mk_i32 16) +. (b1 <<! mk_i32 8)) +. b0));
+  assert ((b2 <<! mk_i32 16) == (mk_i32 (pow2 16) *. b2));
+  assert ((b1 <<! mk_i32 8) == (mk_i32 (pow2 8) *. b1));
+  logand_mask_lemma (((mk_i32 (pow2 16) *. b2) +. (mk_i32 (pow2 8) *. b1)) +. b0) 23;
+  assert (((((mk_i32 (pow2 16) *. b2) +. ((mk_i32 (pow2 8) *. b1)) +. b0)) %! mk_i32 (pow2 23)) ==
+    ((((mk_i32 (pow2 16) *. b2) %! mk_i32 (pow2 23)) +. ((mk_i32 (pow2 8) *. b1)) +. b0)));
+  assert (((((mk_i32 (pow2 16) *. b2) +. (mk_i32 (pow2 8) *. b1)) +. b0) %! mk_i32 (pow2 23)) ==
+    (((mk_i32 (pow2 16) *. (b2 %! mk_i32 128)) +. (mk_i32 (pow2 8) *. b1)) +. b0));
+  assert (((((mk_i32 (pow2 16) *. b2) +. (mk_i32 (pow2 8) *. b1)) +. b0) %! mk_i32 (pow2 23)) ==
+    (((mk_i32 (pow2 16) *. b2') +. (mk_i32 (pow2 8) *. b1)) +. b0))
+
+#pop-options"#
+)]
 #[inline(always)]
-#[hax_lib::fstar::verification_status(lax)]
-#[hax_lib::requires(fstar!(r#"(Seq.length $randomness) / 3 <= Seq.length $out"#))]
+#[hax_lib::requires(fstar!(r#"Seq.length randomness / 3 <= Lib.IntTypes.max_size_t /\
+    Seq.length $randomness / 3 <= Seq.length $out"#))]
 #[hax_lib::ensures(|result| fstar!(r#"let s = Spec.MLDSA.Math.rejection_sample_field_modulus $randomness in
     v $result <= Seq.length ${out}_future /\ v $result == Seq.length s /\
     Seq.slice ${out}_future 0 (v $result) == s"#))]
 pub fn rejection_sample_less_than_field_modulus(randomness: &[u8], out: &mut [i32]) -> usize {
     let mut sampled = 0;
+    let _out_len = out.len();
+    hax_lib::fstar!(
+        r#"Lib.LoopCombinators.eq_repeati0 0 (Spec.MLDSA.Math.rejection_sample_field_modulus_inner $randomness) Seq.empty"#
+    );
 
-    cloop! {
-        for bytes in randomness.chunks_exact(3) {
-            let b0 = bytes[0] as i32;
-            let b1 = bytes[1] as i32;
-            let b2 = bytes[2] as i32;
+    for i in 0..randomness.len() / 3 {
+        hax_lib::loop_invariant!(|i: usize| {
+            fstar!(r#"
+              v $sampled <= v $i /\
+              Seq.length $out == v $_out_len /\
+              (let samples = Lib.LoopCombinators.repeati (v $i)
+                (Spec.MLDSA.Math.rejection_sample_field_modulus_inner $randomness) Seq.empty in
+              v $sampled == Seq.length samples /\
+              Seq.slice $out 0 (Seq.length samples) == samples)"#
+            )
+        });
+        let b0 = randomness[i * 3] as i32;
+        let b1 = randomness[i * 3 + 1] as i32;
+        let b2 = randomness[i * 3 + 2] as i32;
 
-            let coefficient = ((b2 << 16) | (b1 << 8) | b0) & 0x00_7F_FF_FF;
+        let coefficient = ((b2 << 16) | (b1 << 8) | b0) & 0x00_7F_FF_FF;
+        hax_lib::fstar!(
+            r#"rejection_sample_coefficient_lemma $randomness (v $i);
+            Lib.LoopCombinators.unfold_repeati (v $i + 1) 
+                (Spec.MLDSA.Math.rejection_sample_field_modulus_inner $randomness) Seq.empty (v $i)"#
+        );
 
-            if coefficient < FIELD_MODULUS {
-                out[sampled] = coefficient;
-                sampled += 1;
-            }
+        if coefficient < FIELD_MODULUS {
+            out[sampled] = coefficient;
+            sampled += 1;
         }
+        hax_lib::fstar!(
+            r#"let samples = Lib.LoopCombinators.repeati (v $i + 1)
+                (Spec.MLDSA.Math.rejection_sample_field_modulus_inner $randomness) Seq.empty in
+            Lib.Sequence.eq_intro #i32 #(Seq.length samples) (Seq.slice $out 0 (Seq.length samples)) samples"#
+        );
     }
 
     sampled
 }
 
 #[inline(always)]
-#[hax_lib::fstar::verification_status(lax)]
-#[hax_lib::requires(fstar!(r#"(Seq.length $randomness) * 2 <= Seq.length $out"#))]
+#[hax_lib::fstar::options("--z3rlimit 800 --ext context_pruning --z3refresh")]
+#[hax_lib::requires(fstar!(r#"Seq.length randomness * 2 <= Lib.IntTypes.max_size_t /\
+    Seq.length $randomness * 2 <= Seq.length $out"#))]
 #[hax_lib::ensures(|result| fstar!(r#"let s = Spec.MLDSA.Math.rejection_sample_eta_2 $randomness in
     v $result <= Seq.length ${out}_future /\ v $result == Seq.length s /\
     Seq.slice ${out}_future 0 (v $result) == s"#))]
 pub fn rejection_sample_less_than_eta_equals_2(randomness: &[u8], out: &mut [i32]) -> usize {
     let mut sampled = 0;
+    let _out_len = out.len();
+    hax_lib::fstar!(
+        r#"Lib.LoopCombinators.eq_repeati0 0 (Spec.MLDSA.Math.rejection_sample_eta_2_inner $randomness) Seq.empty"#
+    );
 
-    cloop! {
-        for byte in randomness.iter() {
-            let try_0 = byte & 0xF;
-            let try_1 = byte >> 4;
+    for i in 0..randomness.len() {
+        hax_lib::loop_invariant!(|i: usize| {
+            fstar!(r#"
+              v $i >= 0 /\ v $i <= Seq.length $randomness /\
+              v $sampled <= v $i * 2 /\
+              Seq.length $out == v $_out_len /\
+              (let samples = Lib.LoopCombinators.repeati (v $i)
+                (Spec.MLDSA.Math.rejection_sample_eta_2_inner $randomness) Seq.empty in
+              v $sampled == Seq.length samples /\
+              Seq.slice $out 0 (Seq.length samples) == samples)"#
+            )
+        });
+        let byte = randomness[i];
+        let try_0 = byte & 0xF;
+        let try_1 = byte >> 4;
+        hax_lib::fstar!(
+            r#"Lib.LoopCombinators.unfold_repeati (v $i + 1) 
+                (Spec.MLDSA.Math.rejection_sample_eta_2_inner $randomness) Seq.empty (v $i)"#
+        );
 
-            if try_0 < 15 {
-                let try_0 = try_0 as i32;
+        if try_0 < 15 {
+            let try_0 = try_0 as i32;
 
-                // (try_0 * 26) >> 7 computes ⌊try_0 / 5⌋
-                let try_0_mod_5 = try_0 - ((try_0 * 26) >> 7) * 5;
+            // (try_0 * 26) >> 7 computes ⌊try_0 / 5⌋
+            let try_0_mod_5 = try_0 - ((try_0 * 26) >> 7) * 5;
+            hax_lib::fstar!(
+                r#"assert ($try_0_mod_5 == ($try_0 %! mk_i32 5));
+                assert ((mk_i32 2 -. $try_0_mod_5) == (mk_i32 2 -! $try_0_mod_5))"#
+            );
 
-                out[sampled] = 2 - try_0_mod_5;
+            out[sampled] = 2 - try_0_mod_5;
 
-                sampled += 1;
-            }
-
-            if try_1 < 15 {
-                let try_1 = try_1 as i32;
-                let try_1_mod_5 = try_1 - ((try_1 * 26) >> 7) * 5;
-
-                out[sampled] = 2 - try_1_mod_5;
-
-                sampled += 1;
-            }
+            sampled += 1;
         }
+
+        if try_1 < 15 {
+            let try_1 = try_1 as i32;
+            let try_1_mod_5 = try_1 - ((try_1 * 26) >> 7) * 5;
+            hax_lib::fstar!(
+                r#"assert ($try_1_mod_5 == ($try_1 %! mk_i32 5));
+                assert ((mk_i32 2 -. $try_1_mod_5) == (mk_i32 2 -! $try_1_mod_5))"#
+            );
+
+            out[sampled] = 2 - try_1_mod_5;
+
+            sampled += 1;
+        }
+        hax_lib::fstar!(
+            r#"let samples = Lib.LoopCombinators.repeati (v $i + 1)
+                (Spec.MLDSA.Math.rejection_sample_eta_2_inner $randomness) Seq.empty in
+            Lib.Sequence.eq_intro #i32 #(Seq.length samples) (Seq.slice $out 0 (Seq.length samples)) samples"#
+        );
     }
 
     sampled
 }
 
 #[inline(always)]
-#[hax_lib::fstar::verification_status(lax)]
-#[hax_lib::requires(fstar!(r#"(Seq.length $randomness) * 2 <= Seq.length $out"#))]
+#[hax_lib::fstar::options("--ext context_pruning --z3refresh")]
+#[hax_lib::requires(fstar!(r#"Seq.length randomness * 2 <= Lib.IntTypes.max_size_t /\
+    Seq.length $randomness * 2 <= Seq.length $out"#))]
 #[hax_lib::ensures(|result| fstar!(r#"let s = Spec.MLDSA.Math.rejection_sample_eta_4 $randomness in
     v $result <= Seq.length ${out}_future /\ v $result == Seq.length s /\
     Seq.slice ${out}_future 0 (v $result) == s"#))]
 pub fn rejection_sample_less_than_eta_equals_4(randomness: &[u8], out: &mut [i32]) -> usize {
     let mut sampled = 0;
+    let _out_len = out.len();
+    hax_lib::fstar!(
+        r#"Lib.LoopCombinators.eq_repeati0 0 (Spec.MLDSA.Math.rejection_sample_eta_4_inner $randomness) Seq.empty"#
+    );
 
-    cloop! {
-        for byte in randomness.iter() {
-            let try_0 = byte & 0xF;
-            let try_1 = byte >> 4;
+    for i in 0..randomness.len() {
+        hax_lib::loop_invariant!(|i: usize| {
+            fstar!(r#"
+              v $i >= 0 /\ v $i <= Seq.length $randomness /\
+              v $sampled <= v $i * 2 /\
+              Seq.length $out == v $_out_len /\
+              (let samples = Lib.LoopCombinators.repeati (v $i)
+                (Spec.MLDSA.Math.rejection_sample_eta_4_inner $randomness) Seq.empty in
+              v $sampled == Seq.length samples /\
+              Seq.slice $out 0 (Seq.length samples) == samples)"#
+            )
+        });
+        let byte = randomness[i];
+        let try_0 = byte & 0xF;
+        let try_1 = byte >> 4;
+        hax_lib::fstar!(
+            r#"Lib.LoopCombinators.unfold_repeati (v $i + 1) 
+                (Spec.MLDSA.Math.rejection_sample_eta_4_inner $randomness) Seq.empty (v $i)"#
+        );
 
-            if try_0 < 9 {
-                out[sampled] = 4 - (try_0 as i32);
-                sampled += 1;
-            }
-
-            if try_1 < 9 {
-                out[sampled] = 4 - (try_1 as i32);
-                sampled += 1;
-            }
+        if try_0 < 9 {
+            out[sampled] = 4 - (try_0 as i32);
+            sampled += 1;
         }
+
+        if try_1 < 9 {
+            out[sampled] = 4 - (try_1 as i32);
+            sampled += 1;
+        }
+        hax_lib::fstar!(
+            r#"let samples = Lib.LoopCombinators.repeati (v $i + 1)
+                (Spec.MLDSA.Math.rejection_sample_eta_4_inner $randomness) Seq.empty in
+            Lib.Sequence.eq_intro #i32 #(Seq.length samples) (Seq.slice $out 0 (Seq.length samples)) samples"#
+        );
     }
 
     sampled
