libcrux-ml-dsa/proofs/fstar/spec/Spec.MLDSA.Math.fst
@@ -6,8 +6,15 @@ open Core
 let rejection_sample_coefficient (randomness:Seq.seq u8) (i:nat{i < (Seq.length randomness) / 3}) : Tot (i32) =
   let b0 = cast (Seq.index randomness (i * 3)) <: i32 in
   let b1 = cast (Seq.index randomness (i * 3 + 1)) <: i32 in
-  let b2 = cast ((Seq.index randomness (i * 3 + 2)) &. mk_u8 127) <: i32 in
-  ((mk_i32 (pow2 16) *! b2) +! (mk_i32 (pow2 8) *! b1)) +! b0
+  let b2 = cast (Seq.index randomness (i * 3 + 2)) <: i32 in
+  let b2' = if b2 >. mk_i32 127 then b2 -. mk_i32 128  else b2 in
+  ((mk_i32 (pow2 16) *. b2') +. (mk_i32 (pow2 8) *. b1)) +. b0
+
+let rejection_sample_field_modulus_inner1
+  (randomness:Seq.seq u8)
+  (i:nat{i < (Seq.length randomness) / 3})
+  s : (Seq.seq i32) =
+  s
 
 let rejection_sample_field_modulus_inner
   (randomness:Seq.seq u8)
@@ -29,9 +36,9 @@ let rejection_sample_eta_2_inner
   let try_0 = byte &. mk_u8 15 in
   let try_1 = byte >>! mk_u8 4 in
   let s = if try_0 <. mk_u8 15 then 
-    Seq.append s (Seq.create 1 (mk_i32 2 -! ((cast try_0 <: i32) %! mk_i32 5))) else s in
+    Seq.append s (Seq.create 1 (mk_i32 2 -. ((cast try_0 <: i32) %! mk_i32 5))) else s in
   if try_1 <. mk_u8 15 then 
-    Seq.append s (Seq.create 1 (mk_i32 2 -! ((cast try_1 <: i32) %! mk_i32 5))) else s
+    Seq.append s (Seq.create 1 (mk_i32 2 -. ((cast try_1 <: i32) %! mk_i32 5))) else s
 
 let rejection_sample_eta_2 (randomness:Seq.seq u8) : (Seq.seq i32) =
   Lib.LoopCombinators.repeati (Seq.length randomness)
@@ -45,9 +52,9 @@ let rejection_sample_eta_4_inner
   let try_0 = byte &. mk_u8 15 in
   let try_1 = byte >>! mk_u8 4 in
   let s = if try_0 <. mk_u8 9 then 
-    Seq.append s (Seq.create 1 (mk_i32 4 -! (cast try_0 <: i32))) else s in
+    Seq.append s (Seq.create 1 (mk_i32 4 -. (cast try_0 <: i32))) else s in
   if try_1 <. mk_u8 9 then 
-    Seq.append s (Seq.create 1 (mk_i32 4 -! (cast try_1 <: i32))) else s
+    Seq.append s (Seq.create 1 (mk_i32 4 -. (cast try_1 <: i32))) else s
 
 let rejection_sample_eta_4 (randomness:Seq.seq u8) : (Seq.seq i32) =
   Lib.LoopCombinators.repeati (Seq.length randomness)
