libcrux-ml-dsa/proofs/fstar/extraction/Libcrux_ml_dsa.Simd.Portable.Sample.fsti
@@ -4,10 +4,37 @@ open Core
 open FStar.Mul
 
 val rejection_sample_less_than_field_modulus (randomness: t_Slice u8) (out: t_Slice i32)
-    : Prims.Pure (t_Slice i32 & usize) Prims.l_True (fun _ -> Prims.l_True)
+    : Prims.Pure (t_Slice i32 & usize)
+      (requires
+        Seq.length randomness / 3 <= Lib.IntTypes.max_size_t /\
+        Seq.length randomness / 3 <= Seq.length out)
+      (ensures
+        fun temp_0_ ->
+          let out_future, result:(t_Slice i32 & usize) = temp_0_ in
+          let s = Spec.MLDSA.Math.rejection_sample_field_modulus randomness in
+          v result <= Seq.length out_future /\ v result == Seq.length s /\
+          Seq.slice out_future 0 (v result) == s)
 
 val rejection_sample_less_than_eta_equals_2_ (randomness: t_Slice u8) (out: t_Slice i32)
-    : Prims.Pure (t_Slice i32 & usize) Prims.l_True (fun _ -> Prims.l_True)
+    : Prims.Pure (t_Slice i32 & usize)
+      (requires
+        Seq.length randomness * 2 <= Lib.IntTypes.max_size_t /\
+        Seq.length randomness * 2 <= Seq.length out)
+      (ensures
+        fun temp_0_ ->
+          let out_future, result:(t_Slice i32 & usize) = temp_0_ in
+          let s = Spec.MLDSA.Math.rejection_sample_eta_2 randomness in
+          v result <= Seq.length out_future /\ v result == Seq.length s /\
+          Seq.slice out_future 0 (v result) == s)
 
 val rejection_sample_less_than_eta_equals_4_ (randomness: t_Slice u8) (out: t_Slice i32)
-    : Prims.Pure (t_Slice i32 & usize) Prims.l_True (fun _ -> Prims.l_True)
+    : Prims.Pure (t_Slice i32 & usize)
+      (requires
+        Seq.length randomness * 2 <= Lib.IntTypes.max_size_t /\
+        Seq.length randomness * 2 <= Seq.length out)
+      (ensures
+        fun temp_0_ ->
+          let out_future, result:(t_Slice i32 & usize) = temp_0_ in
+          let s = Spec.MLDSA.Math.rejection_sample_eta_4 randomness in
+          v result <= Seq.length out_future /\ v result == Seq.length s /\
+          Seq.slice out_future 0 (v result) == s)
